Tree specs WIP.

specs/Spec.Tree.fst
@@ -32,7 +32,7 @@ let height_gt_one t =
       assert_norm(height (left t) >= 1)
   | Leaf _ _ _ -> ()
 
-#set-options "--z3refresh --z3rlimit 512 --fuel 2 --ifuel 2"
+#set-options "--z3refresh --z3rlimit 512 --fuel 2 --ifuel 2 --z3seed 11"
 let rec leaf_count_gt_height t h =
   match height t with
   | 0 -> ()
@@ -217,6 +217,13 @@ let decode_append (r: root) (a b: seq bool) (sym: nat): Lemma
   | None -> None)) =
   do_decode_append r r a b sym
 
+#push-options "--fuel 2 --ifuel 2"
+let seq_create_tail_eq (#t: Type) (s: seq t): Lemma
+  (requires Seq.length s > 0)
+  (ensures create 1 (head s) @| tail s == s) =
+  let s' = create 1 (head s) @| tail s in assert(equal s s')
+#pop-options
+
 let rec encode_decode_cancel r s =
   code_do_decode_cancel r r s.[0];
   if Seq.length s > 1 then begin
@@ -225,7 +232,9 @@ let rec encode_decode_cancel r s =
   end else
     ();
   match (decode r (encode r s)) with
-  | Some res -> assert(equal s res)
+  | Some res ->
+    seq_create_tail_eq s;
+    assert(equal s res)
   | None -> ()
 
 let rec code_height t s =
@@ -247,56 +256,63 @@ let rec symbol_seq_len_aux t =
     if Leaf? (right t) then () else symbol_seq_len_aux (right t)
 
 #set-options "--z3refresh --z3rlimit 512 --fuel 1 --ifuel 1"
-let rec leftmost_code_vec t =
+let rec leftmost_code_vec t depth =
   match height t with
   | 1 -> ()
   | _ ->
     let l = left t in
     let h = (symbol_seq t).[0] in
-    if Leaf? l then
+    if depth = 1 then
       ()
     else begin
-      leftmost_code_vec l;
-      assert(equal ((create 1 false) @| code l h) (BV.zero_vec #(code_len t h)))
+      leftmost_code_vec l (depth - 1);
+      assert(equal
+        (create 1 false @| code_partial l h (depth - 1))
+        (BV.zero_vec #depth))
     end
 
 #set-options "--z3refresh --z3rlimit 512 --fuel 2 --ifuel 2"
-let rec rightmost_code_vec t =
+let rec rightmost_code_vec t depth =
   match height t with
   | 1 -> ()
   | _ ->
     let r = right t in
     let e = last (symbol_seq t) in
-    if Leaf? r then
+    if depth = 1 then
       ()
     else begin
-      rightmost_code_vec r;
-      assert(equal ((create 1 true) @| code r e) (BV.ones_vec #(code_len t e)))
+      rightmost_code_vec r (depth - 1);
+      assert(equal
+        (create 1 true @| code_partial r e (depth - 1))
+        (BV.ones_vec #depth))
     end
 
 #set-options "--z3refresh --z3rlimit 2048 --fuel 1 --ifuel 1 --z3seed 14"
-let rec code_partial_next t i depth =
+let rec code_partial_next t i =
   match height t with
   | 1 -> ()
   | _ ->
     let l = left t in let r = right t in
     let ts = symbol_seq t in
+    let (s, s') = (ts.[i], ts.[i + 1]) in
     let ls = symbol_seq l in let rs = symbol_seq r in
     let zero = BV.zero_vec #1 in
     let one = BV.ones_vec #1 in
+    let depth = code_len t ts.[i] in
+    let depth' = depth - 1 in
     calc (==) {
-      ((pow2 1) - 1) * pow2 (depth - 1);
+      ((pow2 1) - 1) * pow2 depth';
       =={assert_norm((pow2 1) - 1 == 1)}
-      pow2 (depth - 1);
+      pow2 depth';
     };
-    Math.pow2_double_mult (depth - 1);
+    Math.pow2_double_mult depth';
 
     if depth = 1 then
       ()
     else if i + 1 < total_leaf_count l then begin
-      zero_prefix_vec 1 (code_partial l ls.[i] (depth - 1));
-      zero_prefix_vec 1 (code_partial l ls.[i + 1] (depth - 1));
-      code_partial_next l i (depth - 1)
+      zero_prefix_vec 1 (code_partial l ls.[i] depth');
+      zero_prefix_vec 1 (code_partial l ls.[i + 1] depth');
+      code_partial_next l i
     end else if total_leaf_count l <= i then
       let i' = i - total_leaf_count l in
       calc (==) {
@@ -304,15 +320,13 @@ let rec code_partial_next t i depth =
         =={}
         UInt.from_vec #depth (one @| code r rs.[i']) + 1;
         =={one_prefix_vec 1 (code r rs.[i'])}
-        pow2 (depth - 1) +
-        (UInt.from_vec (code r rs.[i']) + 1);
-        =={code_partial_next r i' (depth - 1)}
-        pow2 (depth - 1) +
-        UInt.from_vec (code r rs.[i' + 1]);
-        =={one_prefix_vec 1 (code r rs.[i' + 1])}
-        UInt.from_vec #depth (one @| code r rs.[i' + 1]);
+        pow2 depth' + (UInt.from_vec (code r rs.[i']) + 1);
+        =={code_partial_next r i'}
+        pow2 depth' + UInt.from_vec (code_partial r rs.[i' + 1] depth');
+        =={one_prefix_vec 1 (code_partial r rs.[i' + 1] depth')}
+        UInt.from_vec #depth (one @| code_partial r rs.[i' + 1] depth');
         =={}
-        UInt.from_vec (code t ts.[i + 1]);
+        UInt.from_vec (code_partial t ts.[i + 1] depth);
       }
     else
       calc (==) {
@@ -321,46 +335,374 @@ let rec code_partial_next t i depth =
         UInt.from_vec #depth (zero @| code l ls.[i]) + 1;
         =={symbol_seq_len_aux l}
         UInt.from_vec #depth (zero @| code l (last ls)) + 1;
-        =={rightmost_code_val l}
+        =={rightmost_code_val l depth'}
         pow2 (code_len l (last ls));
         =={}
-        pow2 (depth - 1);
+        pow2 depth';
         =={UInt.pow2_from_vec_lemma #depth 0}
         UInt.from_vec (BV.elem_vec #depth 0);
         =={
-          leftmost_code_vec r;
-          assert(equal (BV.elem_vec #depth 0) (one @| code r rs.[0]))
+          leftmost_code_vec r depth';
+          assert(equal (BV.elem_vec #depth 0) (one @| code_partial r rs.[0] depth'))
         }
-        UInt.from_vec #depth (one @| code r rs.[0]);
+        UInt.from_vec #depth (one @| code_partial r rs.[0] depth');
         =={}
-        UInt.from_vec (code t ts.[i + 1]);
+        UInt.from_vec (code_partial t ts.[i + 1] depth);
       }
 
-let rec kraft_sum_non_root t =
-  match t with
-  | Internal _ len l r ->
-    calc (=$) {
-      kraft_sum t;
-      =={}
-      kraft_sum l +$ kraft_sum r;
-      =${
-        kraft_sum_non_root l;
-        kraft_sum_non_root r
-      }
-      kraft_term (len + 1) +$ kraft_term (len + 1);
+#push-options "--fuel 0 --ifuel 0"
+let total_leaf_count_aux (t: non_leaf) (i n: int): Lemma
+  (requires i <= total_leaf_count t - n)
+  (ensures i - total_leaf_count (left t) <= total_leaf_count (right t) - n) = ()
+#pop-options
+
+let height_lt (t: non_leaf): Lemma
+  (ensures height (left t) < height t /\ height (right t) < height t)
+  [SMTPatOr [
+    [SMTPat (height (left t))];
+    [SMTPat (height (right t))]
+  ]] = ()
+
+let code_len_subtree (t: non_leaf) (s: tree_symbol t): Lemma
+  (ensures
+    (mem s (symbol_seq (left t)) ==>
+      (Leaf? (left t) ==> code_len t s == 1) /\
+      (Leaf? (left t) == false ==> code_len t s == 1 + code_len (left t) s)) /\
+    (mem s (symbol_seq (right t)) ==> 
+     (Leaf? (right t) ==> code_len t s == 1) /\
+     (Leaf? (right t) == false ==> code_len t s == 1 + code_len (right t) s)))
+  [SMTPatOr [
+    [SMTPat (code_len (left t) s)];
+    [SMTPat (code_len (right t) s)];
+    [SMTPat (code_len t s)]
+  ]] = ()
+
+#push-options "--z3seed 131 --fuel 1 --ifuel 1"
+let rec non_rightmost_upper_bound t i =
+  match height t with
+  | 1 -> ()
+  | _ ->
+    let s = (symbol_seq t).[i] in
+    let l = left t in let r = right t in
+    let ls = symbol_seq l in let rs = symbol_seq r in
+    let depth = code_len t s in
+    if depth = 1 then
+      assert_norm(UInt.from_vec (code t s) == 0)
+    else if mem s ls then begin
+      if Leaf? l then
+        assert(code_len t s == 1)
+      else begin
+        zero_prefix_vec 1 (code l s);
+        Math.pow2_lt_compat depth (depth - 1);
+        assert(i < total_leaf_count l);
+        if i = total_leaf_count l - 1 then 
+          rightmost_code_val l (code_len l s)
+        else
+          non_rightmost_upper_bound l i
+      end
+    end else
+      if Leaf? r then
+        assert(code_len t s == 1)
+      else begin
+        let i' = i - total_leaf_count l in
+        total_leaf_count_aux t i 2;
+        code_len_subtree t s;
+        non_rightmost_upper_bound r i';
+        one_prefix_vec 1 (code r s);
+        assert_norm(pow2 1 - 1 == 1);
+        Math.mul_one_left_is_same (pow2 (depth - 1));
+        Math.pow2_double_sum (depth - 1)
+      end
+#pop-options
+
+let rec code_len_lt_aux t i =
+  match height t with
+  | 1 -> ()
+  | _ ->
+    let (s, s') = ((symbol_seq t).[i], (symbol_seq t).[i + 1]) in
+    let (l, ls) = (left t, symbol_seq (left t)) in
+    if Seq.mem s' ls then
+      ()
+    else
+      let (r, rs) = (right t, symbol_seq (right t)) in
+      if Seq.mem s rs then begin
+        total_leaf_count_aux t i 1;
+        code_len_lt_aux r (i - total_leaf_count l)
+      end else
+        ()
+
+let rec code_len_upper_bound t i =
+  let s = (symbol_seq t).[i] in
+  match height t with
+  | 1 -> ()
+  | _ ->
+    let l = left t in let ls = symbol_seq l in
+    if mem s (symbol_seq (left t)) then
+      if Leaf? l then () else code_len_upper_bound l i
+    else
+      let r = right t in let rs = symbol_seq r in
+      if Leaf? r then () else code_len_upper_bound r (i - total_leaf_count l)
+
+let code_upper_bound t i =
+  let s = (symbol_seq t).[i] in
+  code_len_upper_bound t i;
+  Math.pow2_le_compat (height t) (code_len t s);
+  if i <= total_leaf_count t - 2 then
+    non_rightmost_upper_bound t i
+  else
+    rightmost_code_val t (code_len t s)
+
+let total_leaf_count_left_aux (t: non_leaf) (i: nat): Lemma
+  (requires i < total_leaf_count (left t))
+  (ensures
+    mem (symbol_seq t).[i] (symbol_seq (left t)) /\
+    (Leaf? (left t) == false ==> 
+      code t (symbol_seq t).[i] ==
+      BV.zero_vec #1 @| code (left t) (symbol_seq t).[i])) = ()
+
+let total_leaf_count_right_aux (t: non_leaf) (i: nat): Lemma
+  (requires i < total_leaf_count t /\ total_leaf_count (left t) <= i)
+  (ensures
+    mem (symbol_seq t).[i] (symbol_seq (right t)) /\
+    (Leaf? (right t) == false ==>
+      code t (symbol_seq t).[i] ==
+      BV.ones_vec #1 @| code (right t) (symbol_seq t).[i])) = ()
+
+let symbol_seq_left_index (t: non_leaf) (i: nat): Lemma
+  (requires
+    i < total_leaf_count (left t) /\
+    mem (symbol_seq t).[i] (symbol_seq (left t)))
+  (ensures (symbol_seq (left t)).[i] == (symbol_seq t).[i]) = ()
+
+let symbol_seq_right_index (t: non_leaf) (i: nat): Lemma
+  (requires
+    i < total_leaf_count t /\ total_leaf_count (left t) <= i /\
+    mem (symbol_seq t).[i] (symbol_seq (right t)))
+  (ensures (symbol_seq (right t)).[i - total_leaf_count (left t)] == (symbol_seq t).[i]) = ()
+
+#set-options "--z3refresh --z3rlimit 4096 --fuel 0 --ifuel 0 --z3seed 13"
+let uint_t_code_left (t: non_leaf) (n: pos{n >= height t})  (i: nat): Lemma
+  (requires Leaf? (left t) == false /\ i < Seq.length (symbol_seq (left t)))
+  (ensures uint_t_code t n i == uint_t_code (left t) n i) =
+  let s = (symbol_seq t).[i] in
+  let l = left t in
+  let depth = code_len t s in
+  total_leaf_count_left_aux t i;
+  symbol_seq_left_index t i;
+  if n > depth then begin
+    append_assoc (BV.zero_vec #(n - depth)) (BV.zero_vec #1) (code l s);
+    assert(equal
+      (BV.zero_vec #(n - depth) @| BV.zero_vec #1)
+      (BV.zero_vec #(n - depth + 1)))
+  end else
+    ()
+
+let uint_t_code_right (t: non_leaf) (n: pos{n >= height t}) (i: nat): Lemma
+  (requires
+    Leaf? (right t) == false /\
+    i < total_leaf_count t /\ i >= total_leaf_count (left t))
+  (ensures 
+    uint_t_code t n i ==
+      pow2 (code_len (right t) (symbol_seq (right t)).[i - total_leaf_count (left t)]) +
+      uint_t_code (right t) n (i - total_leaf_count (left t))) =
+  let s = (symbol_seq t).[i] in
+  let (l, r) = (left t, right t) in
+  let depth = code_len t s in
+  let i' = i - total_leaf_count l in
+  total_leaf_count_right_aux t i;
+  symbol_seq_right_index t i;
+  if n > depth then begin
+    calc (==) {
+      UInt.from_vec #n (BV.zero_vec #(n - depth) @| (BV.ones_vec #1 @| code r s));
+      =={zero_prefix_vec (n - depth) (BV.ones_vec #1 @| code r s)}
+      UInt.from_vec #depth (BV.ones_vec #1 @| code r s);
+      =={one_prefix_vec 1 (code r s)}
+      pow2 (depth - 1) + UInt.from_vec (code r s);
     };
-    calc (=$) {
-      kraft_term (len + 1) +$ kraft_term (len + 1);
-      =${
-        assert_norm(len + 1 - 1 == len);
-        kraft_term_plus (len + 1)
-      }
-      kraft_term len;
-    }
-  | Leaf _ len _ -> ()
+    zero_prefix_vec (n - depth + 1) (code r s)
+  end else
+    ()
 
-let kraft_sum_root t =
-  match t with
-  | Root _ l r ->
-    kraft_sum_non_root l;
-    kraft_sum_non_root r
+let pow2_code_len_aux (t: non_leaf) (i: nat): Lemma
+  (requires
+    i < total_leaf_count t - 1 /\
+    code_len t (symbol_seq t).[i] <= code_len t (symbol_seq t).[i + 1])
+  (ensures
+    pow2 ((code_len t (symbol_seq t).[i + 1]) - 1) ==
+    pow2 ((code_len t (symbol_seq t).[i]) - 1) *
+    pow2 ((code_len t (symbol_seq t).[i + 1]) - (code_len t (symbol_seq t).[i]))) =
+  let s = (symbol_seq t).[i] in
+  let s' = (symbol_seq t).[i + 1] in
+  let depth = code_len t s in
+  let depth' = code_len t s' in
+  let diff = depth' - depth in
+  calc (==) {
+    pow2 (depth' - 1);
+    =={
+      calc (==) {
+        depth - 1 + diff;
+        =={Math.subtraction_is_distributive depth 1 diff}
+        (depth - 1) + diff;
+        =={Math.swap_add_plus_minus depth diff 1}
+        depth + diff - 1;
+        =={}
+        depth + (depth' - depth) - 1;
+        =={}
+        depth - (depth - depth') - 1;
+        =={}
+        depth' - 1;
+      }
+    }
+    pow2 ((depth - 1) + diff);
+    =={Math.pow2_plus (depth - 1) diff}
+    (pow2 (depth - 1)) * pow2 diff;
+  }
+
+let minus_plus (a n: int): Lemma (ensures a - n + n == a) = ()
+
+#push-options "--z3refresh --z3rlimit 4096 --fuel 1 --ifuel 1 --z3seed 414"
+let code_next_aux (t: non_leaf) (n: pos{n >= height t}) (i: nat): Lemma
+  (requires
+    canonical_common_cond t i /\
+    i + 1 == total_leaf_count (left t))
+  (ensures
+    uint_t_code t n i < pow2 n - 1 /\
+    uint_t_code t n (i + 1) ==
+    UInt.shift_left
+      ((uint_t_code t n i) + 1)
+      (code_len t (symbol_seq t).[i + 1] - code_len t (symbol_seq t).[i])) =
+  let s = (symbol_seq t).[i] in let s' = (symbol_seq t).[i + 1] in
+  let depth = code_len t s in let depth' = code_len t s' in
+  let diff = depth' - depth in
+  let l = left t in let r = right t in
+  total_leaf_count_left_aux t i;
+  total_leaf_count_right_aux t (i + 1);
+  if depth = 1 then begin
+    assert(uint_t_code t n i == (pow2 (depth - 1)) - 1)
+  end else begin
+    leftmost_code_vec r (depth' - 1);
+    rightmost_code_vec l (depth - 1);
+    assert(UInt.from_vec (code r s') == 0);
+    if n = depth then
+      calc (==) {
+        uint_t_code t n i;
+        =={}
+        UInt.from_vec (code l s);
+        =={rightmost_code_vec l (depth - 1)}
+        (pow2 (depth - 1)) - 1;
+      }
+    else begin
+      zero_prefix_vec (n - depth) (code t s);
+      zero_prefix_vec 1 (code l s);
+      assert(uint_t_code t n i == (pow2 (depth - 1)) - 1)
+    end
+  end;
+  assert(uint_t_code t n i == (pow2 (depth - 1)) - 1);
+  if depth' = 1 then
+    assert(uint_t_code t n (i + 1) == 1)
+  else begin
+    let c = BV.ones_vec #1 @| code r s' in
+    assert((BV.elem_vec #depth' 0).[0] == 
+      (BV.ones_vec #1 @| BV.zero_vec #(depth' - 1)).[0]);
+    assert(forall i. i > 0 ==>
+      (BV.elem_vec #depth' 0).[i] ==
+      (BV.ones_vec #1 @| BV.zero_vec #(depth' - 1)).[i]);
+    assert(equal
+      (BV.ones_vec #1 @| BV.zero_vec #(depth' - 1))
+      (BV.elem_vec #depth' 0));
+    Math.pow2_lt_compat n (depth - 1);
+    Math.pow2_lt_compat n (depth' - 1);
+    calc (==) {
+      uint_t_code t n (i + 1) <: int;
+      =={}
+      UInt.from_vec #depth' (BV.ones_vec #1 @| code r s') <: int;
+      =={leftmost_code_vec r (depth' - 1)}
+      UInt.from_vec #depth' (BV.ones_vec #1 @| BV.zero_vec #(depth' - 1)) <: int;
+      =={
+        lemma_eq_elim
+          (BV.ones_vec #1 @| BV.zero_vec #(depth' - 1))
+          (BV.elem_vec #depth' 0)
+      }
+      UInt.from_vec #depth' (BV.elem_vec #depth' 0) <: int;
+      =={UInt.pow2_from_vec_lemma #depth' 0}
+      pow2 (depth' - 1) <: int;
+      =={Math.modulo_lemma (pow2 (depth' - 1)) (pow2 n)}
+      pow2 (depth' - 1) % pow2 n <: int;
+      =={pow2_code_len_aux t i}
+      pow2 (depth - 1) * pow2 diff % pow2 n <: int;
+    };
+    UInt.shift_left_value_lemma #n (pow2 (depth - 1)) diff;
+    minus_plus (pow2 (depth - 1)) 1
+  end
+#pop-options
+
+#set-options "--z3refresh --z3rlimit 65536 --fuel 0 --ifuel 0 --z3seed 23" // 10
+let rec code_next t n i =
+  let ts = symbol_seq t in let s = ts.[i] in let s' = ts.[i + 1] in
+  let depth = code_len t s in let depth' = code_len t s' in
+  let diff = depth' - depth in
+  non_rightmost_upper_bound t i;
+  if n > depth then begin
+    Math.pow2_lt_compat n depth;
+    zero_prefix_vec (n - depth) (code t s)
+  end else
+    ();
+  let l = left t in
+  if depth = code_len t s' then
+    code_partial_next t i
+  else if i + 1 < total_leaf_count l then
+    if Leaf? l then
+      ()
+    else begin
+      total_leaf_count_left_aux t i;
+      total_leaf_count_left_aux t (i + 1);
+      symbol_seq_left_index t i;
+      symbol_seq_left_index t (i + 1);
+      code_next l n i;
+      calc (==) {
+        uint_t_code t n (i + 1);
+        =={uint_t_code_left t n (i + 1)}
+        uint_t_code l n (i + 1);
+        =={}
+        UInt.shift_left ((uint_t_code l n i) + 1) diff;
+        =={uint_t_code_left t n i}
+        UInt.shift_left ((uint_t_code t n i) + 1) diff;
+      }
+    end
+  else if total_leaf_count l <= i then
+    let r = right t in 
+    if Leaf? r then
+      ()
+    else begin
+      let i' = i - total_leaf_count l in
+      total_leaf_count_right_aux t i;
+      total_leaf_count_right_aux t (i + 1);
+      symbol_seq_right_index t i;
+      symbol_seq_right_index t (i + 1);
+      code_next r n i';
+      uint_t_code_right t n (i + 1);
+      uint_t_code_right t n i;
+      
+      non_rightmost_upper_bound r i';
+      Math.pow2_plus (depth - 1) diff;
+      Math.lemma_mult_lt_right (pow2 diff) (1 + uint_t_code r n i') (pow2 (depth - 1));
+      pow2_code_len_aux t i;
+      Math.pow2_lt_compat n (depth' - 1);
+      // (1 + uint_t_code r n i') * pow2 diff < pow2 (depth' - 1) < pow2 n
+
+      Math.pow2_lt_compat n (depth - 1);
+      Math.modulo_lemma ((1 + uint_t_code r n i') * pow2 diff) (pow2 n);
+      UInt.shift_left_value_lemma #n (1 + uint_t_code r n i') diff;
+      // uint_t_code r n (i' + 1) == (1 + uint_t_code r n i') * pow2 diff
+      // assert(uint_t_code r n (i' + 1) == (1 + uint_t_code r n i') * pow2 diff);
+
+      pow2_code_len_aux t i;
+      Math.distributivity_add_left
+        (pow2 (depth - 1))
+        (1 + uint_t_code r n i')
+        (pow2 diff);
+      Math.modulo_lemma ((pow2 (depth - 1) + 1 + uint_t_code r n i') * pow2 diff) (pow2 n);
+      UInt.shift_left_value_lemma #n (pow2 (depth - 1) + 1 + uint_t_code r n i') diff
+    end
+  else
+    code_next_aux t n i
